theories/Shared/Libs/DLW/Utils/finite.v
@@ -1,0 +1,212 @@
+(**************************************************************)
+(*   Copyright Dominique Larchey-Wendling [*]                 *)
+(*                                                            *)
+(*                             [*] Affiliation LORIA -- CNRS  *)
+(**************************************************************)
+(*      This file is distributed under the terms of the       *)
+(*         CeCILL v2 FREE SOFTWARE LICENSE AGREEMENT          *)
+(**************************************************************)
+
+Require Import List Arith Lia.
+
+From Undecidability.Shared.Libs.DLW.Utils
+  Require Import utils_tac utils_list utils_nat.
+
+From Undecidability.Shared.Libs.DLW.Wf 
+  Require Import acc_irr.
+
+Set Implicit Arguments.
+
+Section finite.
+
+  Definition finite_t X := { lX | forall x : X, In x lX }.
+  Definition finite X := exists lX, forall x : X, In x lX.
+
+  Fact finite_t_finite X : finite_t X -> finite X.
+  Proof. intros (l & ?); exists l; auto. Qed.
+
+  Definition fin_t X (P : X -> Prop) := { l | forall x, P x <-> In x l }.
+  Definition fin X (P : X -> Prop) := exists l, forall x, P x <-> In x l.
+
+  Fact fin_t_fin X P : @fin_t X P -> fin P.
+  Proof. intros (l & ?); exists l; auto. Qed.
+
+  Fact finite_t_fin_t_eq X : (finite_t X -> fin_t (fun _ : X => True))
+                           * (fin_t (fun _ : X => True) -> finite_t X).
+  Proof.
+    split; intros (l & ?); exists l; firstorder.
+  Qed.
+
+  Fact fin_t_map X Y (f : X -> Y) (P Q : _ -> Prop) : 
+             (forall y, Q y <-> exists x, f x = y /\ P x)
+          -> @fin_t X P
+          -> @fin_t Y Q.
+  Proof.
+    intros H (lP & HP).
+    exists (map f lP).
+    intros x; rewrite in_map_iff, H.
+    firstorder.
+  Qed.
+
+  Fixpoint list_prod X Y (l : list X) (m : list Y) :=
+    match l with
+      | nil  => nil
+      | x::l => map (fun y => (x,y)) m ++ list_prod l m
+    end.
+
+  Fact list_prod_spec X Y l m c : In c (@list_prod X Y l m) <-> In (fst c) l /\ In (snd c) m.
+  Proof.
+    revert c; induction l as [ | x l IHl ]; intros c; simpl; try tauto.
+    rewrite in_app_iff, IHl, in_map_iff; simpl.
+    split.
+    + intros [ (y & <- & ?) | (? & ?) ]; simpl; auto.
+    + intros ([ -> | ] & ? ); destruct c; simpl; firstorder.
+  Qed.
+
+  Fact fin_t_prod X Y (P Q : _ -> Prop) : 
+         @fin_t X P -> @fin_t Y Q -> fin_t (fun c => P (fst c) /\ Q (snd c)).
+  Proof.
+    intros (l & Hl) (m & Hm).
+    exists (list_prod l m); intro; rewrite list_prod_spec, Hl, Hm; tauto.
+  Qed.
+
+  Fact finite_prod X Y : finite X -> finite Y -> finite (X*Y).
+  Proof.
+    intros (l & Hl) (m & Hm); exists (list_prod l m).
+    intros []; apply list_prod_spec; auto.
+  Qed.
+
+  Fact fin_t_sum X Y (P Q : _ -> Prop) :
+         @fin_t X P -> @fin_t Y Q -> fin_t (fun z : X + Y => match z with inl x => P x | inr y => Q y end).
+  Proof.
+    intros (l & Hl) (m & Hm).
+    exists (map inl l ++ map inr m).
+    intros z; rewrite in_app_iff, in_map_iff, in_map_iff.
+    destruct z as [ x | y ]; [ rewrite Hl | rewrite Hm ].
+    + split.
+      * left; exists x; auto.
+      * intros [ (z & E & ?) | (z & C & _) ]; try discriminate; inversion E; subst; auto.
+    + split.
+      * right; exists y; auto.
+      * intros [ (z & C & _) | (z & E & ?) ]; try discriminate; inversion E; subst; auto.
+  Qed.
+
+  Fact finite_t_unit : finite_t unit.
+  Proof. exists (tt::nil); intros []; simpl; auto. Qed.
+
+  Fact finite_t_bool : finite_t bool.
+  Proof. exists (true::false::nil); intros []; simpl; auto. Qed.
+
+  Theorem fin_t_length X n : finite_t X -> fin_t (fun l => @length X l < n).
+  Proof.
+    intros HX.
+    apply finite_t_fin_t_eq in HX.
+    generalize finite_t_unit; intros H1.
+    apply finite_t_fin_t_eq in H1.
+    induction n as [ | n IHn ].
+    + exists nil; intros; split; try lia; intros [].
+    + generalize (fin_t_sum H1 (fin_t_prod HX IHn)).
+      apply fin_t_map with (f := fun c => match c with
+        | inl _     => nil
+        | inr (x,l) => x::l
+      end).
+      intros [ | x l ]; simpl.
+      * split; try lia; exists (inl tt); auto.
+      * split.
+        - intros Hl; exists (inr (x,l)); simpl; msplit 2; auto; lia.
+        - intros ([ [] | (y,m) ] & E & H); try discriminate.
+          simpl in *; inversion E; subst; lia.
+  Qed.
+
+  Theorem finite_t_list X n : finite_t X -> finite_t { l : list X | length l < n }.
+  Proof.
+    intros H; apply (fin_t_length n) in H; revert H; intros (l & Hl).
+    assert (forall x, In x l -> length x < n) as f by (intro; apply Hl).
+    set (g x Hx := exist (fun x => length x < n) x (f x Hx)).
+    exists (list_in_map l g).
+    intros (x & Hx).
+    assert (G : In x l) by (revert Hx; apply Hl).
+    assert (E : Hx = f _ G) by apply lt_pirr.
+    subst Hx; apply In_list_in_map with (f := g).
+  Qed.
+
+  Theorem finite_t_option X : finite_t X -> finite_t (option X).
+  Proof.
+    intros (lX & HX).
+    exists (None :: map Some lX).
+    intros [x|]; simpl; auto.
+    right; apply in_map_iff; exists x; auto.
+  Qed.
+
+  Section dec.
+
+    Variable (X : Type) (P : X -> Prop) (Pdec : forall x, { P x } + { ~ P x }).
+    
+    Theorem fin_t_dec Q : @fin_t X Q -> fin_t (fun x => P x /\ Q x).
+    Proof.
+      intros (l & Hl).
+      exists (filter (fun x => if Pdec x then true else false) l).
+      intros x; rewrite filter_In, <- Hl.
+      destruct (Pdec x); try tauto.
+      split; try tauto.
+      intros []; discriminate.
+    Qed.
+
+  End dec.
+
+  Section list_reif.
+
+    Variable (X Y : Type) (eqX_dec : forall x y : X, { x = y } + { x <> y })
+             (R : X -> Y -> Prop).
+    
+    Theorem list_reif (l : list X) :
+            (forall x, In x l -> exists y, R x y)
+         -> exists f, forall x (Hx : In x l), R x (f x Hx).
+    Proof.
+      induction l as [ | x l IHl ]; intros Hl.
+      + exists (fun x (Hx : @In X x nil) => False_rect Y Hx).
+        intros _ [].
+      + destruct (Hl x) as (y & Hy); simpl; auto.
+        destruct IHl as (f & Hf).
+        * intros; apply Hl; simpl; auto.
+        * assert (forall z, In z (x::l) -> x <> z -> In z l) as H1.
+          { intros z [ -> | ] ?; tauto. }
+          exists (fun z Hz => 
+            match eqX_dec x z with
+              | left   _ => y
+              | right  H => f z (H1 _ Hz H)
+            end).
+          intros z Hz.
+          destruct (eqX_dec x z); subst; auto.
+    Qed.  
+ 
+  End list_reif.
+
+  (** Will be useful to reify total relations into actual functions
+      over finite and discrete domains *)
+
+  Theorem finite_reif X Y R : (forall x y : X, { x = y } + { x <> y })
+                           -> finite X
+                           -> (forall x : X, exists y : Y, R x y)
+                           -> exists f, forall x, R x (f x).
+  Proof.
+    intros H1 (l & H2) H3.
+    destruct list_reif with (1 := H1) (R := R) (l := l)
+      as (f & Hf).
+    + intros; auto.
+    + exists (fun x => f x (H2 x)).
+      intros; auto.
+  Qed.
+
+End finite.
+
+Theorem exists_dec_fin_t X (P Q : X -> Prop) 
+           (Pdec : forall x, { P x } + { ~ P x }) 
+           (HQ : fin_t Q)
+           (HPQ : forall x, P x -> Q x) :
+           { exists x, P x } + { ~ exists x, P x }.
+Proof.
+  generalize (fin_t_dec _ Pdec HQ); intros ([ | x l ] & Hl).
+  + right; intros (x & Hx); apply (Hl x); split; auto.
+  + left; exists x; apply Hl; simpl; auto.
+Qed.
