theories/Shared/Libs/DLW/Vec/fin_quotient.v
@@ -1,0 +1,229 @@
+(**************************************************************)
+(*   Copyright Dominique Larchey-Wendling [*]                 *)
+(*                                                            *)
+(*                             [*] Affiliation LORIA -- CNRS  *)
+(**************************************************************)
+(*      This file is distributed under the terms of the       *)
+(*         CeCILL v2 FREE SOFTWARE LICENSE AGREEMENT          *)
+(**************************************************************)
+
+Require Import List Arith Omega Permutation.
+
+From Undecidability.Shared.Libs.DLW.Utils
+  Require Import utils_list.
+
+From Undecidability.Shared.Libs.DLW.Vec 
+  Require Import pos vec.
+
+From Undecidability.Shared.Libs.DLW.Wf 
+  Require Import measure_ind.
+
+Set Implicit Arguments.
+
+Section list_discrim.
+
+  Variable (X : Type) (P Q : X -> Prop) (PQdec : forall x, { P x } + { Q x}).
+
+  Definition list_discrim l : { lP : _ & { lQ | l ~p lP++lQ /\ Forall P lP /\ Forall Q lQ } }.
+  Proof.
+    induction l as [ | x l (lP & lQ & H1 & H2 & H3) ].
+    + exists nil, nil; simpl; auto.
+    + destruct (PQdec x) as [ H | H ].
+      * exists (x::lP), lQ; repeat split; auto; constructor; auto.
+      * exists lP, (x::lQ); repeat split; auto.
+        apply Permutation_cons_app; auto.
+  Qed.
+
+End list_discrim.
+
+Section fp_quotient.
+
+  Variable (X : Type).
+ 
+  Implicit Type (R : X -> X -> Prop).
+
+  Record fp_quotient R := Mk_finite_partial_quotient {
+    fpq_size : nat;
+    fpq_class : X -> option (pos fpq_size);
+    fpq_repr : pos fpq_size -> X;
+    fpq_eq : forall c, fpq_class (fpq_repr c) = Some c;
+    fpq_None : forall x, ~ R x x <-> fpq_class x = None;
+    fpq_Some : forall x y, R x y <-> fpq_class x = fpq_class y /\ fpq_class x <> None;
+  }.
+
+  Let per R := (forall x y, R x y -> R y x) /\ (forall x y z, R x y -> R y z -> R x z).
+  Let dec R := forall x y, { R x y } + { ~ R x y }.
+
+  Let Some_inj K (x y : K) : Some x = Some y -> x = y.
+  Proof. inversion 1; auto. Qed. 
+  
+  Theorem decibable_PER_fp_quotient l R : 
+            (forall x, R x x <-> exists y, In y l /\ R x y) 
+          -> per R -> dec R -> fp_quotient R.
+  Proof.
+    revert R.
+    induction on l as IHl with measure (length l); intros R Hl (H1 & H2) H3.
+    destruct l as [ | x l ].
+    + exists 0 (fun _ => None) (@pos_O_invert _).
+      * intros p; invert pos p.
+      * intros x; rewrite Hl; split; auto.
+        intros _ (? & [] & _).
+      * intros x y; split.
+        - intros H4. 
+          assert (R x x) as C.
+          { apply H2 with y; auto. }
+          apply Hl in C.
+          destruct C as (? & [] & _).
+        - intros (_ & []); auto.
+    + destruct list_discrim with (P := R x) (Q := fun y => ~ R x y) (l := l)
+        as (lx & m & G1 & G2 & G3).
+      { intro; apply H3. }
+      rewrite Forall_forall in G2, G3.
+      set (T u v := ~ R x u /\ R u v).
+      destruct (IHl m) with (R := T) as [ n cl rp Q1 Q2 Q3 ].
+      * apply Permutation_length in G1; rewrite app_length in G1.
+        simpl; omega.
+      * intros u; unfold T; split.
+        - rewrite Hl.
+          intros (F1 & w & [ -> | F2 ] & F3).
+          ++ apply H1 in F3; tauto.
+          ++ exists w; split; auto.
+             apply Permutation_in with (1 := G1), in_app_or in F2.
+             destruct F2; auto.
+             apply G2 in H.
+             contradict F1.
+             apply H2 with w; auto.
+        - intros (v & F1 & F2 & F3); split; auto.
+          apply H2 with v; auto.
+      * split.
+        - intros u v (F1 & F2); split; auto.
+          contradict F1; apply H2 with v; auto.
+        - intros a b c (F1 & F2) (F3 & F4); split; auto.
+          apply H2 with b; auto.
+      * intros u v; unfold T.
+        destruct (H3 x u); destruct (H3 u v); tauto.
+      * destruct (H3 x x) as [ Hx | Hx ].
+        - set (cl' y := match H3 x y with
+               | left Hy  => Some (pos0)
+               | right Hy => match cl y with
+                 | Some p => Some (pos_nxt p)
+                 | None => None
+               end
+             end).
+          set (rp' p := match pos_S_inv p with
+                | inl _  => x
+                | inr (exist _ q _) => rp q
+              end).
+         exists _ cl' rp'.
+         ++ intros p; invert pos p; unfold cl', rp'; simpl.
+            ** destruct (H3 x x) as [ | [] ]; auto.
+            ** rewrite Q1.
+               destruct (H3 x (rp p)) as [ | H ]; auto.
+               unfold T in Q2.
+               specialize (Q1 p).
+               contradict Q1.
+               rewrite (proj1 (Q2 _)); try tauto; discriminate.
+         ++ intros u; unfold cl'; split.
+            ** intros H; destruct (H3 x u) as [ F1 | F1 ].
+               { contradict H; apply H2 with x; auto. }
+               rewrite (proj1 (Q2 _)); auto.
+               intros (? & ?); tauto.
+            ** destruct (H3 x u) as [ F1 | F1 ]; try discriminate.
+               intros F2 F3.
+               destruct (proj1 (Q3 u u)) as (E & ?).
+               red; auto.
+               destruct (cl u); try discriminate; tauto.
+         ++ intros u v; split.
+            ** intros H. 
+               unfold cl'.
+               destruct (H3 x u) as [ F1 | F1 ].
+               { split; try discriminate.
+                 destruct (H3 x v) as [ F2 | F2 ]; auto.
+                 contradict F2; apply H2 with u; auto. }
+               destruct (H3 x v) as [ F2 | F2 ].
+               { contradict F1; apply H2 with v; auto. }
+               destruct (proj1 (Q3 u v)) as (F3 & F4).
+               { red; auto. }
+               rewrite <- F3.
+               destruct (cl u); auto.
+               split; auto; discriminate.
+            ** intros (F1 & F2); revert F1 F2.
+               unfold cl'.
+               { destruct (H3 x u) as [ F1 | F1 ];
+                 destruct (H3 x v) as [ F2 | F2 ].
+                 + intros _ _; apply H2 with x; auto.
+                 + destruct (cl v); discriminate.
+                 + destruct (cl u); discriminate.
+                 + case_eq (cl u).
+                   2: intros _ _ []; auto.
+                   case_eq (cl v); try discriminate.
+                   intros p Hp q Hq E _; apply Q3.
+                   rewrite Hp, Hq; split; try discriminate.
+                   f_equal.
+                   apply Some_inj, pos_nxt_inj in E; subst; auto. }
+        - exists _ cl rp; auto.
+          ++ intros u; split.
+             ** intros H; apply Q2; unfold T; tauto.
+             ** intros H; apply Q2 in H; contradict H; split; auto.
+                contradict Hx; apply H2 with u; auto.
+          ++ intros u v; split.
+             ** intros H; apply Q3.
+                split; auto.
+                contradict Hx; apply H2 with u; auto.
+             ** intros H; apply Q3 in H; destruct H; auto.
+  Qed.
+
+  Record fin_quotient R := Mk_finite_quotient {
+    fq_size : nat;
+    fq_class : X -> pos fq_size;
+    fq_repr : pos fq_size -> X;
+    fq_surj : forall c, fq_class (fq_repr c) = c;
+    fq_equiv : forall x y, R x y <-> fq_class x = fq_class y }.
+
+  (* We do not need the type to be finite, only the number of
+     equivalent classes need be finite *)
+
+  Theorem decidable_EQUIV_fin_quotient l R :
+             (forall x, R x x)
+          -> (forall x y, R x y -> R y x)
+          -> (forall x y z, R x y -> R y z -> R x z)     (* R is an equivalence *)
+          -> (forall x y, { R x y } + { ~ R x y })       (* R is decidable *)
+          -> (forall x : X, exists y, In y l /\ R x y)   (* finitely many classes *)
+          -> fin_quotient R.
+  Proof.
+    intros H1 H2 H3 H4 H5.
+    destruct (@decibable_PER_fp_quotient l R) 
+      as [ n cl rp Q1 Q2 Q3 ]; simpl; auto.
+    + intros x; split; auto; intros _; exists x; auto.
+    + split; auto.
+    + assert (forall x, { y | cl x = Some y }) as H.
+      { intros x; case_eq (cl x).
+        * intros p; exists p; auto.
+        * intros C; exfalso.
+          apply Q2 in C.
+          apply C; auto. }
+      set (cl' x := proj1_sig (H x)).
+      assert (H' : forall x, cl x = Some (cl' x)).
+      { intros x; apply (proj2_sig (H x)). }
+      generalize cl' H'; clear H cl' H'; intros cl' H.
+      exists n cl' rp.
+      * intro x.
+        generalize (Q1 x); rewrite H.
+        injection 1; auto.
+      * intros x y; rewrite Q3.
+        split.
+        - intros (C1 & _).
+          apply Some_inj; rewrite <- H, <- H; auto.
+        - intros E; rewrite H, H, E; split; auto; discriminate.
+  Qed.
+
+End fp_quotient.
+
+Print fp_quotient.
+Check decibable_PER_fp_quotient.
+Print Assumptions decibable_PER_fp_quotient.
+
+Print fin_quotient.
+Check decidable_EQUIV_fin_quotient.
+Print Assumptions decidable_EQUIV_fin_quotient.
+  
