theories/TRAKHTENBROT/bpcp.v
@@ -1,0 +1,173 @@
+(**************************************************************)
+(*   Copyright Dominique Larchey-Wendling [*]                 *)
+(*                                                            *)
+(*                             [*] Affiliation LORIA -- CNRS  *)
+(**************************************************************)
+(*      This file is distributed under the terms of the       *)
+(*         CeCILL v2 FREE SOFTWARE LICENSE AGREEMENT          *)
+(**************************************************************)
+
+Require Import List Arith Lia.
+
+From Undecidability.Shared.Libs.DLW.Utils
+  Require Import utils_tac utils_list utils_nat finite.
+
+Set Implicit Arguments.
+
+Section dec.
+
+  Variable (X : Type) (eqX_dec : forall x y : X, { x = y } + { x <> y }).
+
+  Fact is_a_head_dec (l t : list X) : { x | l = t++x } + { ~ exists x, l = t++x }.
+  Proof.
+    revert t.
+    induction l as [ | a l IHl ].
+    + intros [ | t ]. 
+      * left; exists nil; auto.
+      * right; intros ([ | ] & ?); discriminate.
+    + intros [ | b t ].
+      * left; exists (a::l); auto.
+      * destruct (eqX_dec a b) as [ -> | C ].
+        - destruct (IHl t) as [ H | C ].
+          ++ left; destruct H as (x & ->).
+              exists x; auto.
+          ++ right; contradict C; destruct C as (x & E).
+             exists x; inversion E; subst; auto.
+        - right; contradict C; destruct C as (? & E); inversion E; auto.
+  Qed.
+ 
+  Fact is_a_tail_dec (l t : list X) : { exists x, x++t = l } + { ~ exists x, x++t = l }.
+  Proof.
+    destruct (is_a_head_dec (rev l) (rev t)) as [ H | H ].
+    + left; destruct H as (x & Hx).
+      exists (rev x).
+      apply f_equal with (f := @rev _) in Hx.
+      rewrite rev_app_distr in Hx.
+      do 2 rewrite rev_involutive in Hx; auto.
+    + right; contradict H.
+      destruct H as (x & Hx); exists (rev x); subst.
+      apply rev_app_distr.
+  Qed.
+
+End dec.
+
+Section pcp_hand.
+
+  Variable (X : Type) (lc : list (list X * list X)).
+
+  Inductive pcp_hand : list X -> list X -> Prop :=
+    | in_pcph_0 : forall x y, In (x,y) lc -> pcp_hand x y
+    | in_pcph_1 : forall x y u l, In (x,y) lc -> pcp_hand u l -> pcp_hand (x++u) (y++l).
+
+  (** Any hand is either a card or of the for x++p/y++q where
+      x/y is a non-void card and p/q is a hand *)
+
+  Lemma pcp_hand_inv p q : 
+       pcp_hand p q -> In (p,q) lc 
+                    \/ exists x y p' q', In (x,y) lc /\ pcp_hand p' q' 
+                                      /\ p = x++p' /\ q = y++q' 
+                        /\  (x <> nil /\ y = nil  
+                          \/ x = nil /\ y <> nil
+                          \/ x <> nil /\ y <> nil ).
+  Proof.
+    induction 1 as [ x y H | x y p q H1 H2 IH2 ].
+    + left; auto. 
+    + destruct x as [ | a x ]; [ destruct y as [ | b y ] | ].
+      * simpl; auto.
+      * right; exists nil, (b::y), p, q; simpl; msplit 4; auto.
+        right; left; split; auto; discriminate.
+      * right; exists (a::x), y, p, q; simpl; msplit 4; auto.
+        destruct y.
+        - left; split; auto; discriminate.
+        - right; right; split; discriminate.
+  Qed.
+
+  Definition PCP := exists l, pcp_hand l l.
+
+  Section pcp_induction.
+
+    Implicit Type (l m : list X).
+
+    (** Notice that we could downgrade strict_suffix to Prop because
+        a and b could be computed from the knowledge of there existence *)
+
+    Definition strict_suffix x y l m := { a : _ & { b | (a <> nil \/ b <> nil) /\ l = a++x /\ m = b++y } }.
+    
+    Variable (P : list X -> list X -> Type)
+             (IHP : forall l m, (forall l' m', strict_suffix l' m' l m -> P l' m') -> P l m).
+
+    Theorem pcp_induction l m : P l m.
+    Proof.
+      induction on l m as IH with measure (length l + length m).
+      apply IHP.
+      intros l' m' (x & y & H & -> & ->).
+      apply IH.
+      do 2 rewrite app_length.
+      destruct x; destruct y; simpl; try lia.
+      destruct H as [ [] | [] ]; auto.
+    Qed.
+
+  End pcp_induction.
+    
+  Section bounded_dec.
+
+    (** It is possible to decide pcp_hand, when equality is decidable
+        of course *)
+  
+    Variable eqX_dec : forall x y : X, { x = y } + { x <> y }.
+
+    Let eqlX_dec : forall l m : list X, { l = m } + { l <> m }.
+    Proof. apply list_eq_dec; auto. Qed.
+
+    Let eqXX_dec : forall p q : list X * list X, { p = q } + { p <> q }.
+    Proof. decide equality; auto. Qed.
+
+    (** Replaced induction on length p + length with strict suffix pair induction *)
+
+    Theorem pcp_hand_dec p q : { pcp_hand p q } + { ~ pcp_hand p q }.
+    Proof.
+      revert p q; apply pcp_induction; intros p q dec.
+
+      set (P (c : list X * list X) := let (x,y) := c 
+           in exists d, p = x++fst d /\ q = y++snd d /\ pcp_hand (fst d) (snd d) /\ (x <> nil \/ y <> nil)).
+      assert (forall c, { P c } + { ~ P c }) as Pdec.
+      { intros (x,y); simpl.
+        assert ( { x = nil /\ y = nil } + { x <> nil \/ y <> nil } ) as H.
+        1: { destruct (eqlX_dec x nil); destruct (eqlX_dec y nil); tauto. }
+        destruct H as [ (H1 & H2) | Hxy ].
+        1: { right; intros ((? & ?) & ?); tauto. }
+        destruct (is_a_head_dec eqX_dec p x) as [ (p' & Hp') | Hp ].
+        2: { right; contradict Hp; revert Hp. 
+             intros ((p',?) & E & _); exists p'; auto. }
+        destruct (is_a_head_dec eqX_dec q y) as [ (q' & Hq') | Hq ].
+        2: { right; contradict Hq; revert Hq. 
+             intros ((?,q') & _ & E & _); exists q'; auto. }
+        destruct (dec p' q') as [ H' | H' ].
+        + exists x, y; auto.
+        + left; exists (p',q'); auto.
+        + right; contradict H'; revert H'.
+          intros ((u,v) & -> & -> & C & _); simpl in *.
+          apply app_inv_head in Hp'.
+          apply app_inv_head in Hq'.
+          subst; auto. }
+
+      destruct list_dec with (1 := Pdec) (l := lc)
+        as [ ((x,y) & H1 & H) | H ]; unfold P in H.
+      + left.
+        destruct H as ((p',q') & -> & -> & H & _); simpl in *.
+        constructor 2; auto.
+      + destruct In_dec with (1 := eqXX_dec) (a := (p,q)) (l := lc)
+          as [ H2 | H2 ].
+        * left; constructor 1; auto.
+        * right; contradict H2.
+          apply pcp_hand_inv in H2.
+          destruct H2 as [ | (x & y & p' & q' & H2 & H3 & -> & -> & H4) ]; auto.
+          destruct H with (1 := H2).
+          exists (p', q'); msplit 3; tauto.
+    Qed.
+
+  End bounded_dec.
+
+End pcp_hand.
+
+
