theories/TRAKHTENBROT/fo_logic.v
@@ -1,0 +1,256 @@
+(**************************************************************)
+(*   Copyright Dominique Larchey-Wendling [*]                 *)
+(*                                                            *)
+(*                             [*] Affiliation LORIA -- CNRS  *)
+(**************************************************************)
+(*      This file is distributed under the terms of the       *)
+(*         CeCILL v2 FREE SOFTWARE LICENSE AGREEMENT          *)
+(**************************************************************)
+
+Require Import List Arith Lia.
+
+From Undecidability.Shared.Libs.DLW.Utils
+  Require Import utils_list finite.
+
+From Undecidability.Shared.Libs.DLW.Vec 
+  Require Import pos vec.
+
+From Undecidability.TRAKHTENBROT
+  Require Import notations fol_ops fo_terms.
+
+Set Implicit Arguments.
+
+Notation ø := vec_nil.
+
+Opaque fo_term_subst fo_term_map fo_term_sem.
+
+Record fo_signature := {
+  syms : Type;
+  rels : Type;
+  ar_syms : syms -> nat;
+  ar_rels : rels -> nat
+}.
+
+(** Unscoped (nat) DeBruijn syntax for FOL formulas *)
+
+Inductive fol_form (Σ : fo_signature) : Type :=
+  | fol_false : fol_form Σ
+  | fol_atom  : forall p, vec (fo_term nat (ar_syms Σ)) (ar_rels Σ p) -> fol_form Σ 
+  | fol_bin   : fol_bop -> fol_form Σ -> fol_form Σ -> fol_form Σ 
+  | fol_quant : fol_qop -> fol_form Σ -> fol_form Σ. 
+
+Infix "⤑" := (fol_bin fol_imp) (at level 62, right associativity).
+Infix "⟑" := (fol_bin fol_conj) (at level 60, right associativity).
+Infix "⟇" := (fol_bin fol_disj) (at level 61, right associativity).
+Notation "∀ f" := (fol_quant fol_fa f) (at level 63, right associativity).
+Notation "∃ f" := (fol_quant fol_ex f) (at level 63, right associativity).
+
+Notation "£" := ((@in_var nat _ _) : nat -> fo_term nat _).
+Notation "⊥" := (fol_false _).
+
+Section fol_subst.
+
+  Variable (Σ : fo_signature).
+
+  Notation 𝕋 := (fo_term nat (ar_syms Σ)).
+  Notation 𝔽 := (fol_form Σ).
+
+  (* Notation ⟦ ⟧ ⟪ ⟫ φ ψ σ ρ ↑ ⦃ ⦄ ⇡*)
+
+  Fixpoint fol_vars (A : 𝔽) :=
+    match A with
+      | ⊥              => nil
+      | fol_atom _ p v => flat_map (@fo_term_vars _ _ _) (vec_list v)
+      | fol_bin c A B => fol_vars A ++ fol_vars B
+      | fol_quant q A => flat_map (fun n => match n with 0 => nil | S n => n::nil end)
+                           (fol_vars A) 
+    end.
+
+  Fixpoint fol_subst σ (A : 𝔽) :=
+    match A with
+      | ⊥              => ⊥
+      | fol_atom _ p v => fol_atom _ _ (vec_map (fo_term_subst σ) v)
+      | fol_bin c A B => fol_bin c (A⦃σ⦄) (B⦃σ⦄)
+      | fol_quant q A => fol_quant q (A⦃⇡σ⦄) 
+    end
+  where "A ⦃ σ ⦄" := (fol_subst σ A).
+
+  Fact fol_subst_ext σ ρ A : 
+       (forall n, In n (fol_vars A) -> σ n = ρ n) -> A⦃σ⦄ = A⦃ρ⦄.
+  Proof.
+    intros Hfg; revert A σ ρ Hfg. 
+    induction A as [ | p v | c A IHA B IHB | q A IHA ]; intros f g Hfg; simpl; f_equal; auto.
+    + apply vec_map_ext; intros t Ht. 
+      apply fo_term_subst_ext; intros n Hn.
+      apply Hfg, in_flat_map; exists t; split; auto.
+      apply in_vec_list; auto.
+    + apply IHA; intros n Hn; apply Hfg, in_or_app; auto.
+    + apply IHB; intros n Hn; apply Hfg, in_or_app; auto.
+    + apply IHA; intros [ | n ] Hn; simpl; auto.
+      rew fot.
+      f_equal; apply Hfg; simpl.
+      apply in_flat_map; exists (S n); simpl; auto. 
+  Qed.
+
+  Definition fol_bigop c A := fold_right (@fol_bin Σ c) A.
+
+  Fact fol_subst_bigop c l A σ : (fol_bigop c A l)⦃σ⦄ = fol_bigop c (A⦃σ⦄) (map (fol_subst σ) l).
+  Proof. induction l; simpl; f_equal; auto. Qed.
+
+  (** This theorem is the important one that shows substitutions do compose 
+      hence De Bruijn notation are handled correctly by substitutions *)
+
+  Fact fol_subst_subst σ ρ A : A⦃σ⦄⦃ρ⦄ = A⦃fun n => (σ n)⟬ρ⟭⦄.
+  Proof.
+    revert σ ρ; induction A 
+        as [ | p v | b A IHA B IHB | q A IHA ]; 
+        simpl; intros f g; auto.
+    + f_equal.
+      rewrite vec_map_map.
+      apply vec_map_ext.
+      intros A w; rew fot; auto. 
+    + f_equal; auto.
+    + f_equal.
+      rewrite IHA; auto.
+      apply fol_subst_ext.
+      intros [ | n ] _; rew fot; simpl; rew fot; simpl; auto.
+      do 2 rewrite <- fo_term_subst_map, fo_term_subst_comp.
+      apply fo_term_subst_ext.
+      intros; rew fot; rewrite fo_term_subst_map; simpl; rew fot; auto.
+  Qed.
+
+End fol_subst.
+
+Notation "A ⦃ σ ⦄" := (fol_subst σ A).
+
+Record fo_model Σ := {
+  fom_type :> Type;
+  fom_syms : forall s, vec fom_type (ar_syms Σ s) -> fom_type;
+  fom_rels : forall s, vec fom_type (ar_rels Σ s) -> Prop }.
+
+Section fol_semantics.
+
+  Variable (Σ : fo_signature) (M : fo_model Σ).
+
+  Notation X := (fom_type M).
+  Notation sem_sym := (fom_syms M _).
+  Notation sem_pred := (fom_rels M _).
+
+  Implicit Type φ : nat -> X.
+
+  Notation "⟦ t ⟧" := (fun φ => fo_term_sem (fom_syms M) φ t).
+
+  (* Notation ⟦ ⟧ ⟪ ⟫ φ ψ σ ↑ *)
+
+  Fixpoint fol_sem φ A : Prop :=
+      match A with
+        | ⊥              => False
+        | fol_atom _ _ v => sem_pred (vec_map (fun t => ⟦t⟧ φ) v)
+        | fol_bin b A B  => fol_bin_sem b (⟪A⟫ φ) (⟪B⟫ φ) 
+        | fol_quant q A  => fol_quant_sem q (fun x => ⟪A⟫ (φ↑x))
+      end
+    where "⟪ A ⟫" := (fun φ => fol_sem φ A).
+
+  Definition fol_ldisj := @fol_bigop Σ fol_disj ⊥.
+  Definition fol_lconj := @fol_bigop Σ fol_conj (⊥⤑⊥).
+
+  Fact fol_sem_big_disj lf φ : ⟪ fol_ldisj lf ⟫ φ <-> exists f, In f lf /\ ⟪ f ⟫ φ.
+  Proof.
+    induction lf as [ | f lf IHlf ]; simpl.
+    + split; try tauto; intros ( ? & [] & _).
+    + rewrite IHlf.
+      split.
+      * intros [ H | (g & H1 & H2) ].
+        - exists f; auto.
+        - exists g; auto.
+      * intros (g & [ <- | Hg ] & ?); auto.
+        right; exists g; auto.
+  Qed.
+
+  Fact fol_sem_big_conj lf φ : ⟪ fol_lconj lf ⟫ φ <-> forall f, In f lf -> ⟪ f ⟫ φ.
+  Proof.
+    induction lf as [ | f lf IHlf ]; simpl.
+    + split; tauto.
+    + rewrite IHlf.
+      split.
+      * intros [] ? [ -> | ]; auto.
+      * intros H; split; intros; apply H; auto.
+  Qed.
+
+  (** Semantics depends only on occuring variables *)
+
+  Fact fol_sem_ext φ ψ A : (forall n, In n (fol_vars A) -> φ n = ψ n) -> ⟪A⟫ φ <-> ⟪A⟫ ψ.
+  Proof.
+    intros H; revert A φ ψ H.
+    induction A as [ | p v | b A IHA B IHB | q A IHA ]; simpl; intros phi psy H; try tauto.
+    + match goal with | |- sem_pred ?x <-> sem_pred ?y => replace y with x; try tauto end.
+      apply vec_map_ext; intros w Hw. 
+      apply fo_term_sem_ext; auto.
+      intros n Hn; apply H, in_flat_map; exists w; split; auto.
+      apply in_vec_list; auto.
+    + apply fol_bin_sem_ext.
+      * apply IHA; intros; apply H, in_or_app; auto.
+      * apply IHB; intros; apply H, in_or_app; auto.
+    + apply fol_quant_sem_ext.
+      intros x; apply IHA.
+      intros [ | n] Hn; simpl; auto; apply H, in_flat_map.
+      exists (S n); simpl; auto.
+  Qed.
+
+  (* Notation ⟦ ⟧ ⟪ ⟫ φ ψ σ ↑ ⦃ ⦄*)
+
+  (** Semantics commutes with substitutions ... good *)
+
+  Theorem fol_sem_subst φ σ A : ⟪ A⦃σ⦄ ⟫ φ <-> ⟪A⟫ (fun n => ⟦σ n⟧ φ).
+  Proof.
+    revert φ σ; induction A as [ | p v | b A IHA B IHB | q A IHA ]; simpl; intros phi f; try tauto.
+    + match goal with | |- sem_pred ?x <-> sem_pred ?y => replace y with x; try tauto end.
+      rewrite vec_map_map; apply vec_map_ext.
+      intros; rewrite fo_term_sem_subst; auto.
+    + apply fol_bin_sem_ext; auto.
+    + apply fol_quant_sem_ext.
+      intros x; rewrite IHA.
+      apply fol_sem_ext. 
+      intros [ | n ] _; simpl; rew fot; simpl; auto.
+      rewrite <- fo_term_subst_map; rew fot.
+      apply fo_term_sem_ext; intros; rew fot; auto.
+  Qed.
+
+  Definition fo_model_dec := forall s (v : vec _ (ar_rels _ s)), { sem_pred v } + { ~ sem_pred v }.
+
+  Section decidable.
+
+    (** REMARK: not requiring the sem_pred relation to be decidable
+        would allow hiding uncomputability inside the model which
+        would be kind of cheating. The semantic relation should be
+        decidable, only the (finite) satisfiability relation should 
+        be undec *)
+
+    (** For the semantics relation to be decidable over a finite domain,
+        it is necessary and SUFFICIENT that the sem_pred relation is decidable
+       or equivalently, each predicate is interpreted as a map: vec X _ -> bool *)
+
+    Variable (M_fin : finite_t X).
+    Variable (rels_dec : fo_model_dec).
+
+    Theorem fol_sem_dec A φ : { ⟪A⟫ φ } + { ~ ⟪A⟫ φ }.
+    Proof.
+      revert φ.
+      induction A as [ | p v | b A IHA B IHB | q A IHA ]; intros phi.
+      + simpl; tauto.
+      + simpl; apply rels_dec.
+      + simpl fol_sem; apply fol_bin_sem_dec; auto.
+      + simpl fol_sem; apply fol_quant_sem_dec; auto.
+    Qed.
+
+  End decidable.
+
+End fol_semantics.
+
+(** A first order formula over signature Σ is finitely satisfiable if
+    there exists a model M interpreting the signature Σ which 
+    is both finite (strongly listable) and strongly decidable,
+    and a valuation φ : nat -> M in which A is satisfied *)
+
+Definition fo_form_fin_SAT Σ A := 
+  exists (M : fo_model Σ)  (_ : finite_t M) (_ : fo_model_dec M) φ, fol_sem M φ A.
