theories/TRAKHTENBROT/fol_ops.v
@@ -1,0 +1,76 @@
+(**************************************************************)
+(*   Copyright Dominique Larchey-Wendling [*]                 *)
+(*                                                            *)
+(*                             [*] Affiliation LORIA -- CNRS  *)
+(**************************************************************)
+(*      This file is distributed under the terms of the       *)
+(*         CeCILL v2 FREE SOFTWARE LICENSE AGREEMENT          *)
+(**************************************************************)
+
+Require Import List Arith Lia.
+
+From Undecidability.Shared.Libs.DLW.Utils
+  Require Import utils_list finite.
+
+Set Implicit Arguments.
+
+Inductive fol_bop := fol_conj | fol_disj | fol_imp.
+Inductive fol_qop := fol_ex | fol_fa.
+
+Definition fol_bin_sem b :=
+  match b with
+    | fol_conj => and
+    | fol_disj => or
+    | fol_imp  => fun A B => A -> B
+  end.
+
+Fact fol_bin_sem_ext b A A' B B' :
+     (A <-> A') -> (B <-> B') -> (fol_bin_sem b A B <-> fol_bin_sem b A' B').
+Proof.
+  intros E1 E2; destruct b; simpl; tauto.
+Qed. 
+
+Arguments fol_bin_sem b /.
+
+Fact fol_bin_sem_dec b A B : 
+       { A } + { ~ A } -> { B } + { ~ B } 
+    -> { fol_bin_sem b A B } + { ~ fol_bin_sem b A B }.
+Proof. revert b; intros [] HA HB; simpl; tauto. Qed.
+
+Definition fol_quant_sem X q (P : X -> Prop) :=
+  match q with
+    | fol_ex => ex P
+    | fol_fa => forall x, P x 
+  end.
+
+Arguments fol_quant_sem X q P /.
+
+Fact fol_quant_sem_ext X (P Q : X -> Prop) : 
+        (forall x, P x <-> Q x) 
+      -> forall q, fol_quant_sem q P <-> fol_quant_sem q Q.
+Proof.
+  intros H []; simpl.
+  + split; intros (k & ?); exists k; apply H; auto.
+  + split; intros ? k; apply H; auto. 
+Qed.
+
+Fact fol_quant_sem_dec X q (P : X -> Prop) : 
+       finite_t X 
+    -> (forall x, { P x } + { ~ P x }) 
+    -> { fol_quant_sem q P } + { ~ fol_quant_sem q P }.
+Proof.
+  intros (lX & HlX). 
+  revert q; intros [] H; simpl.
+  + destruct list_dec with (1 := H) (l := lX)
+      as [ (x & H1 & H2) | H1 ].
+    * left; firstorder.
+    * right; intros (y & Hy).
+      apply (H1 y); auto.
+  + destruct list_dec with (P := fun x => ~ P x) (Q := P) (l := lX)
+      as [ (x & H1 & H2) | H1 ].
+    * firstorder.
+    * right; contradict H2; auto.
+    * left; intros x; apply H1; auto.
+Qed.
+
+
