theories/TRAKHTENBROT/notations.v
@@ -1,0 +1,38 @@
+(**************************************************************)
+(*   Copyright Dominique Larchey-Wendling [*]                 *)
+(*                                                            *)
+(*                             [*] Affiliation LORIA -- CNRS  *)
+(**************************************************************)
+(*      This file is distributed under the terms of the       *)
+(*         CeCILL v2 FREE SOFTWARE LICENSE AGREEMENT          *)
+(**************************************************************)
+
+(* Unicode DB for cut/paste 
+  -> ⇡ ↑ 
+  -> ⟬  ⟭ ⟦ ⟧ ⟪ ⟫ ⦃ ⦄
+  -> φ ψ σ ρ 𝕋 𝔽 
+*)
+
+(** Lifting a term substitution *)
+Reserved Notation "⇡ sig" (at level 1, format "⇡ sig").
+
+(** Lifting a DeBruijn subtitution *)
+Reserved Notation "phi ↑ k" (at level 1, format "phi ↑ k", left associativity).
+
+(** Term substitution and semantics *)
+Reserved Notation "t '⟬' σ '⟭'" (at level 1, format "t ⟬ σ ⟭").
+Reserved Notation "'⟦' t '⟧'" (at level 1, format "⟦ t ⟧").
+
+(** Formula subsitution and semantics*)
+Reserved Notation "f '⦃' σ '⦄'" (at level 1, format "f ⦃ σ ⦄").
+Reserved Notation "'⟪' f '⟫'" (at level 1, format "⟪ f ⟫").
+
+(* A non-recursive fixpoint to get correct unfolding *)
+
+Fixpoint env_lift {X} (φ : nat -> X) k n { struct n } :=
+  match n with
+    | 0   => k
+    | S n => φ n
+  end.
+
+Notation "phi ↑ k" := (env_lift phi k).
